byteback-dummy/java8/src/main/java/byteback/dummy/field/StaticField.java
@@ -1,0 +1,21 @@
+package byteback.dummy.field;
+
+public class StaticField {
+
+	static boolean booleanField;
+
+	static byte byteField;
+
+	static short shortField;
+
+	static int intField;
+
+	static long longField;
+
+	static float floatField;
+
+	static double doubleField;
+
+	static Object referenceField;
+
+}
