byteback-dummy/java8/src/main/java/byteback/dummy/function/Field.java
@@ -4,7 +4,19 @@ import byteback.annotations.Contract.Pure;
 
 public class Field {
 
+	public static int staticField;
+
 	public int field;
+
+	@Pure
+	public int staticFieldReference() {
+		return staticField;
+	}
+
+	@Pure
+	public int staticFieldSum() {
+		return staticField + 2;
+	}
 
 	@Pure
 	public int fieldReference() {
