byteback-core/src/integration/resources/regression/java8/boogie/byteback.dummy.condition.Instance.bpl
@@ -1,0 +1,8 @@
+procedure byteback.dummy.condition.Instance.isObject##()
+{
+	var $stack1 : Reference;
+	call $stack1 := ~new(java.lang.Object);
+	call java.lang.Object.$init$##($stack1);
+	assert ~instanceof(~heap, $stack1, java.lang.Object);
+	return;
+}
