byteback-core/src/integration/resources/regression/java8/boogie/byteback.dummy.field.InstanceField.bpl
@@ -1,0 +1,15 @@
+const unique byteback.dummy.field.InstanceField.booleanField: Field bool;
+
+const unique byteback.dummy.field.InstanceField.byteField: Field int;
+
+const unique byteback.dummy.field.InstanceField.shortField: Field int;
+
+const unique byteback.dummy.field.InstanceField.intField: Field int;
+
+const unique byteback.dummy.field.InstanceField.longField: Field int;
+
+const unique byteback.dummy.field.InstanceField.floatField: Field real;
+
+const unique byteback.dummy.field.InstanceField.doubleField: Field real;
+
+const unique byteback.dummy.field.InstanceField.referenceField: Field Reference;
