byteback-core/src/integration/resources/regression/java8/boogie/byteback.dummy.field.StaticField.bpl
@@ -1,0 +1,15 @@
+const unique byteback.dummy.field.StaticField.booleanField: Field bool;
+
+const unique byteback.dummy.field.StaticField.byteField: Field int;
+
+const unique byteback.dummy.field.StaticField.shortField: Field int;
+
+const unique byteback.dummy.field.StaticField.intField: Field int;
+
+const unique byteback.dummy.field.StaticField.longField: Field int;
+
+const unique byteback.dummy.field.StaticField.floatField: Field real;
+
+const unique byteback.dummy.field.StaticField.doubleField: Field real;
+
+const unique byteback.dummy.field.StaticField.referenceField: Field Reference;
