byteback-core/src/integration/resources/regression/java8/boogie/byteback.dummy.function.Field.bpl
@@ -6,6 +6,16 @@ procedure byteback.dummy.function.Field.$init$##(this: Reference) returns ()
   return;
 }
 
+function byteback.dummy.function.Field.staticFieldReference##(~heap: Store, this: Reference) returns (int)
+{
+   ~read(~heap, byteback.dummy.function.Field, byteback.dummy.function.Field.staticField)
+}
+
+function byteback.dummy.function.Field.staticFieldSum##(~heap: Store, this: Reference) returns (int)
+{
+   ~read(~heap, byteback.dummy.function.Field, byteback.dummy.function.Field.staticField) + 2
+}
+
 function byteback.dummy.function.Field.fieldReference##(~heap: Store, this: Reference) returns (int)
 {
    ~read(~heap, this, byteback.dummy.function.Field.field)
